φ = (1+√5)/2
ψ = (1-√5)/2

[1] φ2 = (1+√5)2/4 = (1 + 2√5 + 5)/4 = (3+√5)/2
[2] ψ2 = (1-√5)2/4 = (3-√5)/2

By induction
Base cases:
Fib(0)= (φ0 – ψ0)/√5 = 0
Fib(1)= (φ – ψ)/√5 = [(1+√5)/2 – (1-√5)/2] / √5 = 1

Induction step:
[3] Fib(k) = (φk – ψk)/√5
[4] Fib(k+1) = (φ.φk – ψ.ψk)/√5
By definition Fib(k+2) = Fib(k) + Fib(k+1)
[3] + [4] Fib(k+2) = [φk(1+φ) – ψk(1+ψ)] / √5
(1+φ) = 1 + (1+√5)/2 = (3+√5)/2 = φ^2 – from [1]
(1+ψ) = 1 + (1-√5)/2 = (3-√5)/2 = ψ^2 – from [2]
Fib(k+2) = φk.φ2 – ψk.ψ2 / √5 = (φk+2 – ψk+2) / √5

Now ψ = (1-√5)/2 and 4 < 5 2 < √5 -1 < ψ ψn -> 0 as n -> ∞
Fib(n) -> (φ – 0)n/√5 as n -> ∞
Fib(n) -> φn/√5